Test Simple Equations
=====================

$\nabla \times \mathbf{E} = - \frac{\partial \mathbf{B}}{\partial t}$

$$\nabla \times \mathbf{E} = - \frac{\partial \mathbf{B}}{\partial t}$$

$\nabla \times \mathbf{E} = - \frac{\partial \mathbf{B}}{\partial t}$

$$\nabla \times \mathbf{E} = - \frac{\partial \mathbf{B}}{\partial t}$$

Test MathJax Environments
=========================

$$\begin{aligned}
\nabla \times \mathbf{E} = - \frac{\partial \mathbf{B}}{\partial t}\end{aligned}$$

$$\begin{aligned}
\nabla \times \mathbf{E} = - \frac{\partial \mathbf{B}}{\partial t}\end{aligned}$$

$$\begin{aligned}
{2}
\nabla \times \mathbf{E} = - \frac{\partial \mathbf{B}}{\partial t}\end{aligned}$$

$$\begin{aligned}
{2}
\nabla \times \mathbf{E} = - \frac{\partial \mathbf{B}}{\partial t}\end{aligned}$$

$$\begin{aligned}
\nabla \times \mathbf{E} = - \frac{\partial \mathbf{B}}{\partial t}
\end{aligned}$$

$$\begin{alignedat}{2}
\nabla \times \mathbf{E} = - \frac{\partial \mathbf{B}}{\partial t}
\end{alignedat}$$

$$\begin{array}{lcl}
\nabla \times \mathbf{E} = - \frac{\partial \mathbf{B}}{\partial t}
\end{array}$$

$$\begin{Bmatrix}
\nabla \times \mathbf{E} = - \frac{\partial \mathbf{B}}{\partial t}
\end{Bmatrix}$$

$$\begin{bmatrix}
\nabla \times \mathbf{E} = - \frac{\partial \mathbf{B}}{\partial t}
\end{bmatrix}$$

$$\begin{cases}
\nabla \times \mathbf{E} = - \frac{\partial \mathbf{B}}{\partial t}
\end{cases}$$

$$\begin{CD}
\nabla \times \mathbf{E} = - \frac{\partial \mathbf{B}}{\partial t}
\end{CD}$$

$$\begin{aligned}
\nabla \times \mathbf{E} = - \frac{\partial \mathbf{B}}{\partial t}\end{aligned}$$

$$\begin{aligned}
\nabla \times \mathbf{E} = - \frac{\partial \mathbf{B}}{\partial t}\end{aligned}$$

$$\nabla \times \mathbf{E} = - \frac{\partial \mathbf{B}}{\partial t}$$

$$\nabla \times \mathbf{E} = - \frac{\partial \mathbf{B}}{\partial t}$$

$$\begin{gathered}
\nabla \times \mathbf{E} = - \frac{\partial \mathbf{B}}{\partial t}\end{gathered}$$

$$\begin{gathered}
\nabla \times \mathbf{E} = - \frac{\partial \mathbf{B}}{\partial t}\end{gathered}$$

$$\begin{gathered}
\nabla \times \mathbf{E} = - \frac{\partial \mathbf{B}}{\partial t}
\end{gathered}$$

$$\begin{matrix}
\nabla \times \mathbf{E} = - \frac{\partial \mathbf{B}}{\partial t}
\end{matrix}$$

$$\begin{gathered}
\nabla \times \mathbf{E} = - \frac{\partial \mathbf{B}}{\partial t}\end{gathered}$$

$$\begin{gathered}
\nabla \times \mathbf{E} = - \frac{\partial \mathbf{B}}{\partial t}\end{gathered}$$

$$\begin{pmatrix}
\nabla \times \mathbf{E} = - \frac{\partial \mathbf{B}}{\partial t}
\end{pmatrix}$$

$$\begin{smallmatrix}
\nabla \times \mathbf{E} = - \frac{\partial \mathbf{B}}{\partial t}
\end{smallmatrix}$$

$$\begin{split}
\nabla \times \mathbf{E} = - \frac{\partial \mathbf{B}}{\partial t}
\end{split}$$

$$\begin{subarray}
\nabla \times \mathbf{E} = - \frac{\partial \mathbf{B}}{\partial t}
\end{subarray}$$

$$\begin{Vmatrix}
\nabla \times \mathbf{E} = - \frac{\partial \mathbf{B}}{\partial t}
\end{Vmatrix}$$

$$\begin{vmatrix}
\nabla \times \mathbf{E} = - \frac{\partial \mathbf{B}}{\partial t}
\end{vmatrix}$$
