\documentclass[]{article}
\usepackage{lmodern}
\usepackage{amssymb,amsmath}
\usepackage{ifxetex,ifluatex}
\usepackage{fixltx2e} % provides \textsubscript
\ifnum 0\ifxetex 1\fi\ifluatex 1\fi=0 % if pdftex
  \usepackage[T1]{fontenc}
  \usepackage[utf8]{inputenc}
\else % if luatex or xelatex
  \ifxetex
    \usepackage{mathspec}
  \else
    \usepackage{fontspec}
  \fi
  \defaultfontfeatures{Ligatures=TeX,Scale=MatchLowercase}
\fi
% use upquote if available, for straight quotes in verbatim environments
\IfFileExists{upquote.sty}{\usepackage{upquote}}{}
% use microtype if available
\IfFileExists{microtype.sty}{%
\usepackage{microtype}
\UseMicrotypeSet[protrusion]{basicmath} % disable protrusion for tt fonts
}{}
\usepackage{hyperref}
\hypersetup{unicode=true,
            pdfborder={0 0 0},
            breaklinks=true}
\urlstyle{same}  % don't use monospace font for urls
\IfFileExists{parskip.sty}{%
\usepackage{parskip}
}{% else
\setlength{\parindent}{0pt}
\setlength{\parskip}{6pt plus 2pt minus 1pt}
}
\setlength{\emergencystretch}{3em}  % prevent overfull lines
\providecommand{\tightlist}{%
  \setlength{\itemsep}{0pt}\setlength{\parskip}{0pt}}
\setcounter{secnumdepth}{0}
% Redefines (sub)paragraphs to behave more like sections
\ifx\paragraph\undefined\else
\let\oldparagraph\paragraph
\renewcommand{\paragraph}[1]{\oldparagraph{#1}\mbox{}}
\fi
\ifx\subparagraph\undefined\else
\let\oldsubparagraph\subparagraph
\renewcommand{\subparagraph}[1]{\oldsubparagraph{#1}\mbox{}}
\fi

\date{}

\begin{document}

\section{Test Simple Equations}\label{test-simple-equations}

\(\nabla \times \mathbf{E} = - \frac{\partial \mathbf{B}}{\partial t}\)

\[\nabla \times \mathbf{E} = - \frac{\partial \mathbf{B}}{\partial t}\]

\section{Test MathJax Environments}\label{test-mathjax-environments}

\begin{align}
\nabla \times \mathbf{E} = - \frac{\partial \mathbf{B}}{\partial t}
\end{align}

\begin{align*}
\nabla \times \mathbf{E} = - \frac{\partial \mathbf{B}}{\partial t}
\end{align*}

\begin{alignat}{2}
\nabla \times \mathbf{E} = - \frac{\partial \mathbf{B}}{\partial t}
\end{alignat}

\begin{alignat*}{2}
\nabla \times \mathbf{E} = - \frac{\partial \mathbf{B}}{\partial t}
\end{alignat*}

\[\begin{aligned}
\nabla \times \mathbf{E} = - \frac{\partial \mathbf{B}}{\partial t}
\end{aligned}\]

\[\begin{alignedat}{2}
\nabla \times \mathbf{E} = - \frac{\partial \mathbf{B}}{\partial t}
\end{alignedat}\]

\[\begin{array}{lcl}
\nabla \times \mathbf{E} = - \frac{\partial \mathbf{B}}{\partial t}
\end{array}\]

\[\begin{Bmatrix}
\nabla \times \mathbf{E} = - \frac{\partial \mathbf{B}}{\partial t}
\end{Bmatrix}\]

\[\begin{bmatrix}
\nabla \times \mathbf{E} = - \frac{\partial \mathbf{B}}{\partial t}
\end{bmatrix}\]

\[\begin{cases}
\nabla \times \mathbf{E} = - \frac{\partial \mathbf{B}}{\partial t}
\end{cases}\]

\[\begin{CD}
\nabla \times \mathbf{E} = - \frac{\partial \mathbf{B}}{\partial t}
\end{CD}\]

\begin{eqnarray}
\nabla \times \mathbf{E} = - \frac{\partial \mathbf{B}}{\partial t}
\end{eqnarray}

\begin{eqnarray*}
\nabla \times \mathbf{E} = - \frac{\partial \mathbf{B}}{\partial t}
\end{eqnarray*}

\begin{equation}
\nabla \times \mathbf{E} = - \frac{\partial \mathbf{B}}{\partial t}
\end{equation}

\begin{equation*}
\nabla \times \mathbf{E} = - \frac{\partial \mathbf{B}}{\partial t}
\end{equation*}

\begin{gather}
\nabla \times \mathbf{E} = - \frac{\partial \mathbf{B}}{\partial t}
\end{gather}

\begin{gather*}
\nabla \times \mathbf{E} = - \frac{\partial \mathbf{B}}{\partial t}
\end{gather*}

\[\begin{gathered}
\nabla \times \mathbf{E} = - \frac{\partial \mathbf{B}}{\partial t}
\end{gathered}\]

\[\begin{matrix}
\nabla \times \mathbf{E} = - \frac{\partial \mathbf{B}}{\partial t}
\end{matrix}\]

\begin{multline}
\nabla \times \mathbf{E} = - \frac{\partial \mathbf{B}}{\partial t}
\end{multline}

\begin{multline*}
\nabla \times \mathbf{E} = - \frac{\partial \mathbf{B}}{\partial t}
\end{multline*}

\[\begin{pmatrix}
\nabla \times \mathbf{E} = - \frac{\partial \mathbf{B}}{\partial t}
\end{pmatrix}\]

\[\begin{smallmatrix}
\nabla \times \mathbf{E} = - \frac{\partial \mathbf{B}}{\partial t}
\end{smallmatrix}\]

\[\begin{split}
\nabla \times \mathbf{E} = - \frac{\partial \mathbf{B}}{\partial t}
\end{split}\]

\[\begin{subarray}
\nabla \times \mathbf{E} = - \frac{\partial \mathbf{B}}{\partial t}
\end{subarray}\]

\[\begin{Vmatrix}
\nabla \times \mathbf{E} = - \frac{\partial \mathbf{B}}{\partial t}
\end{Vmatrix}\]

\[\begin{vmatrix}
\nabla \times \mathbf{E} = - \frac{\partial \mathbf{B}}{\partial t}
\end{vmatrix}\]

\end{document}
