\documentclass{article}
\usepackage{amsmath}
\usepackage{amscd}
\begin{document}

\section{Test Simple Equations}

$\nabla \times \mathbf{E} = - \frac{\partial \mathbf{B}}{\partial t}$

$$\nabla \times \mathbf{E} = - \frac{\partial \mathbf{B}}{\partial t}$$

\(\nabla \times \mathbf{E} = - \frac{\partial \mathbf{B}}{\partial t}\)

\[\nabla \times \mathbf{E} = - \frac{\partial \mathbf{B}}{\partial t}\]

\section{Test MathJax Environments}

\begin{align}
\nabla \times \mathbf{E} = - \frac{\partial \mathbf{B}}{\partial t}
\end{align}

\begin{align*}
\nabla \times \mathbf{E} = - \frac{\partial \mathbf{B}}{\partial t}
\end{align*}

\begin{alignat}{2}
\nabla \times \mathbf{E} = - \frac{\partial \mathbf{B}}{\partial t}
\end{alignat}

\begin{alignat*}{2}
\nabla \times \mathbf{E} = - \frac{\partial \mathbf{B}}{\partial t}
\end{alignat*}

\[
\begin{aligned}
\nabla \times \mathbf{E} = - \frac{\partial \mathbf{B}}{\partial t}
\end{aligned}
\]

\[
\begin{alignedat}{2}
\nabla \times \mathbf{E} = - \frac{\partial \mathbf{B}}{\partial t}
\end{alignedat}
\]

\[
\begin{array}{lcl}
\nabla \times \mathbf{E} = - \frac{\partial \mathbf{B}}{\partial t}
\end{array}
\]

\[
\begin{Bmatrix}
\nabla \times \mathbf{E} = - \frac{\partial \mathbf{B}}{\partial t}
\end{Bmatrix}
\]

\[
\begin{bmatrix}
\nabla \times \mathbf{E} = - \frac{\partial \mathbf{B}}{\partial t}
\end{bmatrix}
\]

\[
\begin{cases}
\nabla \times \mathbf{E} = - \frac{\partial \mathbf{B}}{\partial t}
\end{cases}
\]

\[
\begin{CD}
\nabla \times \mathbf{E} = - \frac{\partial \mathbf{B}}{\partial t}
\end{CD}
\]

\begin{eqnarray}
\nabla \times \mathbf{E} = - \frac{\partial \mathbf{B}}{\partial t}
\end{eqnarray}

\begin{eqnarray*}
\nabla \times \mathbf{E} = - \frac{\partial \mathbf{B}}{\partial t}
\end{eqnarray*}

\begin{equation}
\nabla \times \mathbf{E} = - \frac{\partial \mathbf{B}}{\partial t}
\end{equation}

\begin{equation*}
\nabla \times \mathbf{E} = - \frac{\partial \mathbf{B}}{\partial t}
\end{equation*}

\begin{gather}
\nabla \times \mathbf{E} = - \frac{\partial \mathbf{B}}{\partial t}
\end{gather}

\begin{gather*}
\nabla \times \mathbf{E} = - \frac{\partial \mathbf{B}}{\partial t}
\end{gather*}

\[
\begin{gathered}
\nabla \times \mathbf{E} = - \frac{\partial \mathbf{B}}{\partial t}
\end{gathered}
\]

\[
\begin{matrix}
\nabla \times \mathbf{E} = - \frac{\partial \mathbf{B}}{\partial t}
\end{matrix}
\]

\begin{multline}
\nabla \times \mathbf{E} = - \frac{\partial \mathbf{B}}{\partial t}
\end{multline}

\begin{multline*}
\nabla \times \mathbf{E} = - \frac{\partial \mathbf{B}}{\partial t}
\end{multline*}

\[
\begin{pmatrix}
\nabla \times \mathbf{E} = - \frac{\partial \mathbf{B}}{\partial t}
\end{pmatrix}
\]

\[
\begin{smallmatrix}
\nabla \times \mathbf{E} = - \frac{\partial \mathbf{B}}{\partial t}
\end{smallmatrix}
\]

\[
\begin{split}
\nabla \times \mathbf{E} = - \frac{\partial \mathbf{B}}{\partial t}
\end{split}
\]

\[
\begin{subarray}
\nabla \times \mathbf{E} = - \frac{\partial \mathbf{B}}{\partial t}
\end{subarray}
\]

\[
\begin{Vmatrix}
\nabla \times \mathbf{E} = - \frac{\partial \mathbf{B}}{\partial t}
\end{Vmatrix}
\]

\[
\begin{vmatrix}
\nabla \times \mathbf{E} = - \frac{\partial \mathbf{B}}{\partial t}
\end{vmatrix}
\]

\end{document}